\section{Covariant J Alternative}\label{appendix-1}
If we use equation \ref{cl-cross-co} , we need to find covariant components of $\J$ too, which are as shown above,

\begin{align}
    J_\rho = \J \cdot \e_\rho = (J^\rho \e_\rho + J^\theta \e_\theta + J^\zeta \e_\zeta) \cdot \e_\rho \\
    J_\theta = \J \cdot \e_\theta = (J^\rho \e_\rho + J^\theta \e_\theta + J^\zeta \e_\zeta) \cdot \e_\theta \\
    J_\zeta = \J \cdot \e_\zeta = (J^\rho \e_\rho + J^\theta \e_\theta + J^\zeta \e_\zeta) \cdot \e_\zeta
\end{align}
Hence,
\begin{align}
    \J \times \B &= \frac{1}{\sqrt{g}} \sum_k (J_i B_j - J_j B_i)\e_k \\
    &= \frac{1}{\sqrt{g}} \begin{bmatrix}
        (J_\theta B_\zeta - J_\zeta B_\theta)\e_\rho  \hspace{.2cm}+\hspace{.2cm}
        (J_\zeta B_\rho - J_\rho B_\zeta)\e_\theta    \hspace{.2cm}+\hspace{.2cm}
        (J_\rho B_\theta - J_\theta B_\rho)\e_\zeta
    \end{bmatrix}
\end{align}